<USER>
### 7. On the Plus Side

X X X X X X

Place all the numbers 1, 2, 3, 4, 5, and 7 in the boxes in such a way that the first number is smaller than the last, and in every set of three consecutive boxes, there are two numbers and their sum.

<ASSISTANT>
### Understanding the Problem

The puzzle presents six boxes arranged in a row:

```
X X X X X X
```

We are to place the numbers **1, 2, 3, 4, 5,** and **7** into these boxes under the following conditions:

1. **First Number is Smaller than the Last:** The number in the first box must be less than the number in the last box.
2. **Triplet Sum Condition:** In every set of three consecutive boxes, there are two numbers whose sum equals the third number.

Our goal is to determine the correct sequence of numbers that satisfies both conditions.

### Breaking Down the Conditions

Let's analyze each condition to understand what constraints they impose on the sequence.

#### Condition 1: First Number < Last Number

This is straightforward. If we denote the sequence as \( a_1, a_2, a_3, a_4, a_5, a_6 \), then:

\[ a_1 < a_6 \]

This means that whatever number we place in the first box must be smaller than the number in the last box.

#### Condition 2: Triplet Sum Condition

This condition is more complex. For every set of three consecutive boxes, the numbers must satisfy the relationship where one number is the sum of the other two.

In other words, for any triplet \( (a_i, a_{i+1}, a_{i+2}) \), one of the following must be true:

1. \( a_i + a_{i+1} = a_{i+2} \)
2. \( a_i + a_{i+2} = a_{i+1} \)
3. \( a_{i+1} + a_{i+2} = a_i \)

This condition must hold for all possible triplets in the sequence, which are:

- \( (a_1, a_2, a_3) \)
- \( (a_2, a_3, a_4) \)
- \( (a_3, a_4, a_5) \)
- \( (a_4, a_5, a_6) \)

### Strategy for Solving the Puzzle

Given these conditions, here's how I plan to approach the problem:

1. **List All Possible Numbers:** We have the numbers 1, 2, 3, 4, 5, and 7 to place in the boxes.
2. **Determine Possible Pairs and Their Sums:** Since in every triplet, one number is the sum of the other two, it's helpful to list all possible pairs and their sums to see which combinations are feasible.
3. **Start with the First Box:** Since the first number must be smaller than the last, starting with the smallest number might be advantageous.
4. **Build the Sequence Step by Step:** After placing the first number, use the triplet condition to determine the next numbers, ensuring that each new number satisfies the conditions with its predecessors.
5. **Check for Consistency:** At each step, verify that the sequence so far adheres to both conditions.
6. **Backtrack if Necessary:** If a dead end is reached, backtrack to the previous step and try a different number.

### Step 1: Listing All Possible Numbers

We have the numbers: **1, 2, 3, 4, 5, 7**.

### Step 2: Determining Possible Pairs and Their Sums

Let's list all possible pairs and their sums:

- \( 1 + 2 = 3 \)
- \( 1 + 3 = 4 \)
- \( 1 + 4 = 5 \)
- \( 1 + 5 = 6 \) (Note: 6 is not in our list)
- \( 1 + 7 = 8 \) (Not in our list)
- \( 2 + 3 = 5 \)
- \( 2 + 4 = 6 \) (Not in our list)
- \( 2 + 5 = 7 \)
- \( 2 + 7 = 9 \) (Not in our list)
- \( 3 + 4 = 7 \)
- \( 3 + 5 = 8 \) (Not in our list)
- \( 3 + 7 = 10 \) (Not in our list)
- \( 4 + 5 = 9 \) (Not in our list)
- \( 4 + 7 = 11 \) (Not in our list)
- \( 5 + 7 = 12 \) (Not in our list)

From this, the valid pairs and their sums within our number set are:

- \( 1 + 2 = 3 \)
- \( 1 + 3 = 4 \)
- \( 1 + 4 = 5 \)
- \( 2 + 3 = 5 \)
- \( 2 + 5 = 7 \)
- \( 3 + 4 = 7 \)

These are the only combinations where the sum is also one of the numbers we have to place.

### Step 3: Starting with the First Box

Given that the first number must be smaller than the last, starting with the smallest number, **1**, seems logical.

Let's tentatively place **1** in the first box:

```
1 X X X X X
```

Now, we need to determine the second number. Let's consider the first triplet: \( (a_1, a_2, a_3) = (1, a_2, a_3) \).

According to the triplet condition, one of the following must be true:

1. \( 1 + a_2 = a_3 \)
2. \( 1 + a_3 = a_2 \)
3. \( a_2 + a_3 = 1 \)

However, since all our numbers are positive integers greater than or equal to 1, the third option \( a_2 + a_3 = 1 \) is impossible because the smallest sum we can have is \( 1 + 1 = 2 \).

So, we're left with:

1. \( 1 + a_2 = a_3 \)
2. \( 1 + a_3 = a_2 \)

Let's explore both possibilities.

#### Option 1: \( 1 + a_2 = a_3 \)

If \( a_3 = 1 + a_2 \), then \( a_3 \) must be greater than \( a_2 \).

Given our available numbers (2, 3, 4, 5, 7), let's see possible pairs:

- If \( a_2 = 2 \), then \( a_3 = 3 \)
- If \( a_2 = 3 \), then \( a_3 = 4 \)
- If \( a_2 = 4 \), then \( a_3 = 5 \)
- If \( a_2 = 5 \), then \( a_3 = 6 \) (But 6 is not in our list)
- If \( a_2 = 7 \), then \( a_3 = 8 \) (Not in our list)

So, the valid pairs for \( (a_2, a_3) \) are:

- \( (2, 3) \)
- \( (3, 4) \)
- \( (4, 5) \)

Let's explore each of these possibilities.

##### Sub-option 1: \( a_2 = 2 \), \( a_3 = 3 \)

Sequence so far:

```
1 2 3 X X X
```

Now, consider the next triplet: \( (a_2, a_3, a_4) = (2, 3, a_4) \).

Applying the triplet condition:

1. \( 2 + 3 = 5 \), so \( a_4 = 5 \)
2. \( 2 + a_4 = 3 \) ⇒ \( a_4 = 1 \) (But 1 is already used)
3. \( 3 + a_4 = 2 \) ⇒ \( a_4 = -1 \) (Invalid)

Thus, the only valid option is \( a_4 = 5 \).

Sequence now:

```
1 2 3 5 X X
```

Next triplet: \( (a_3, a_4, a_5) = (3, 5, a_5) \).

Applying the triplet condition:

1. \( 3 + 5 = 8 \) (Not in our list)
2. \( 3 + a_5 = 5 \) ⇒ \( a_5 = 2 \) (But 2 is already used)
3. \( 5 + a_5 = 3 \) ⇒ \( a_5 = -2 \) (Invalid)

This leads to a dead end because there's no valid number for \( a_5 \). Therefore, the initial assumption \( a_2 = 2 \), \( a_3 = 3 \) does not yield a valid sequence.

##### Sub-option 2: \( a_2 = 3 \), \( a_3 = 4 \)

Sequence so far:

```
1 3 4 X X X
```

Next triplet: \( (a_2, a_3, a_4) = (3, 4, a_4) \).

Applying the triplet condition:

1. \( 3 + 4 = 7 \), so \( a_4 = 7 \)
2. \( 3 + a_4 = 4 \) ⇒ \( a_4 = 1 \) (Already used)
3. \( 4 + a_4 = 3 \) ⇒ \( a_4 = -1 \) (Invalid)

Thus, \( a_4 = 7 \).

Sequence now:

```
1 3 4 7 X X
```

Next triplet: \( (a_3, a_4, a_5) = (4, 7, a_5) \).

Applying the triplet condition:

1. \( 4 + 7 = 11 \) (Not in our list)
2. \( 4 + a_5 = 7 \) ⇒ \( a_5 = 3 \) (Already used)
3. \( 7 + a_5 = 4 \) ⇒ \( a_5 = -3 \) (Invalid)

Again, we reach a dead end. Therefore, \( a_2 = 3 \), \( a_3 = 4 \) does not work.

##### Sub-option 3: \( a_2 = 4 \), \( a_3 = 5 \)

Sequence so far:

```
1 4 5 X X X
```

Next triplet: \( (a_2, a_3, a_4) = (4, 5, a_4) \).

Applying the triplet condition:

1. \( 4 + 5 = 9 \) (Not in our list)
2. \( 4 + a_4 = 5 \) ⇒ \( a_4 = 1 \) (Already used)
3. \( 5 + a_4 = 4 \) ⇒ \( a_4 = -1 \) (Invalid)

This also leads to a dead end. Therefore, \( a_2 = 4 \), \( a_3 = 5 \) is invalid.

#### Conclusion from Option 1

None of the sub-options under Option 1 (\( 1 + a_2 = a_3 \)) yielded a valid sequence. Therefore, we need to explore Option 2.

#### Option 2: \( 1 + a_3 = a_2 \)

If \( a_2 = 1 + a_3 \), then \( a_2 \) must be greater than \( a_3 \).

Given our available numbers (2, 3, 4, 5, 7), let's see possible pairs:

- If \( a_3 = 2 \), then \( a_2 = 3 \)
- If \( a_3 = 3 \), then \( a_2 = 4 \)
- If \( a_3 = 4 \), then \( a_2 = 5 \)
- If \( a_3 = 5 \), then \( a_2 = 6 \) (Not in our list)
- If \( a_3 = 7 \), then \( a_2 = 8 \) (Not in our list)

So, the valid pairs for \( (a_2, a_3) \) are:

- \( (3, 2) \)
- \( (4, 3) \)
- \( (5, 4) \)

Let's explore each of these possibilities.

##### Sub-option 1: \( a_2 = 3 \), \( a_3 = 2 \)

Sequence so far:

```
1 3 2 X X X
```

Next triplet: \( (a_2, a_3, a_4) = (3, 2, a_4) \).

Applying the triplet condition:

1. \( 3 + 2 = 5 \), so \( a_4 = 5 \)
2. \( 3 + a_4 = 2 \) ⇒ \( a_4 = -1 \) (Invalid)
3. \( 2 + a_4 = 3 \) ⇒ \( a_4 = 1 \) (Already used)

Thus, \( a_4 = 5 \).

Sequence now:

```
1 3 2 5 X X
```

Next triplet: \( (a_3, a_4, a_5) = (2, 5, a_5) \).

Applying the triplet condition:

1. \( 2 + 5 = 7 \), so \( a_5 = 7 \)
2. \( 2 + a_5 = 5 \) ⇒ \( a_5 = 3 \) (Already used)
3. \( 5 + a_5 = 2 \) ⇒ \( a_5 = -3 \) (Invalid)

Thus, \( a_5 = 7 \).

Sequence now:

```
1 3 2 5 7 X
```

Next triplet: \( (a_4, a_5, a_6) = (5, 7, a_6) \).

Applying the triplet condition:

1. \( 5 + 7 = 12 \) (Not in our list)
2. \( 5 + a_6 = 7 \) ⇒ \( a_6 = 2 \) (Already used)
3. \( 7 + a_6 = 5 \) ⇒ \( a_6 = -2 \) (Invalid)

This leads to a dead end. Therefore, \( a_2 = 3 \), \( a_3 = 2 \) does not yield a valid sequence.

##### Sub-option 2: \( a_2 = 4 \), \( a_3 = 3 \)

Sequence so far:

```
1 4 3 X X X
```

Next triplet: \( (a_2, a_3, a_4) = (4, 3, a_4) \).

Applying the triplet condition:

1. \( 4 + 3 = 7 \), so \( a_4 = 7 \)
2. \( 4 + a_4 = 3 \) ⇒ \( a_4 = -1 \) (Invalid)
3. \( 3 + a_4 = 4 \) ⇒ \( a_4 = 1 \) (Already used)

Thus, \( a_4 = 7 \).

Sequence now:

```
1 4 3 7 X X
```

Next triplet: \( (a_3, a_4, a_5) = (3, 7, a_5) \).

Applying the triplet condition:

1. \( 3 + 7 = 10 \) (Not in our list)
2. \( 3 + a_5 = 7 \) ⇒ \( a_5 = 4 \) (Already used)
3. \( 7 + a_5 = 3 \) ⇒ \( a_5 = -4 \) (Invalid)

This also leads to a dead end. Therefore, \( a_2 = 4 \), \( a_3 = 3 \) is invalid.

##### Sub-option 3: \( a_2 = 5 \), \( a_3 = 4 \)

Sequence so far:

```
1 5 4 X X X
```

Next triplet: \( (a_2, a_3, a_4) = (5, 4, a_4) \).

Applying the triplet condition:

1. \( 5 + 4 = 9 \) (Not in our list)
2. \( 5 + a_4 = 4 \) ⇒ \( a_4 = -1 \) (Invalid)
3. \( 4 + a_4 = 5 \) ⇒ \( a_4 = 1 \) (Already used)

This leads to a dead end. Therefore, \( a_2 = 5 \), \( a_3 = 4 \) does not work.

#### Conclusion from Option 2

None of the sub-options under Option 2 (\( 1 + a_3 = a_2 \)) yielded a valid sequence either.

### Re-evaluating Our Approach

Since starting with **1** in the first box did not lead to a valid sequence, perhaps we need to consider starting with a different number. Let's try starting with **2**.

### Starting with 2 in the First Box

Let's tentatively place **2** in the first box:

```
2 X X X X X
```

Now, we need to determine the second number. Let's consider the first triplet: \( (a_1, a_2, a_3) = (2, a_2, a_3) \).

Applying the triplet condition:

1. \( 2 + a_2 = a_3 \)
2. \( 2 + a_3 = a_2 \)
3. \( a_2 + a_3 = 2 \)

Again, since all numbers are at least 1, the third option \( a_2 + a_3 = 2 \) is impossible because the smallest sum is \( 1 + 1 = 2 \), but both numbers cannot be 1 (as we have only one '1').

So, we're left with:

1. \( 2 + a_2 = a_3 \)
2. \( 2 + a_3 = a_2 \)

Let's explore both possibilities.

#### Option 1: \( 2 + a_2 = a_3 \)

If \( a_3 = 2 + a_2 \), then \( a_3 \) must be greater than \( a_2 \).

Given our available numbers (1, 3, 4, 5, 7), let's see possible pairs:

- If \( a_2 = 1 \), then \( a_3 = 3 \)
- If \( a_2 = 3 \), then \( a_3 = 5 \)
- If \( a_2 = 4 \), then \( a_3 = 6 \) (Not in our list)
- If \( a_2 = 5 \), then \( a_3 = 7 \)
- If \( a_